Source/IntegrationTests/TestFiles/LitTests/LitTest/referrers/referrers.bpl
@@ -5440,6 +5440,10 @@ implementation {:smt_option "smt.arith.solver", "2"} {:verboseName "ChainingObje
   var this.nontracking: ref;
   var this.tracking: ref;
   var this.tail: ref;
+  var defass#this.x: bool;
+  var defass#this.y: bool;
+  var defass#this.tracking: bool;
+  var defass#this.tail: bool;
   var $oldRhs: ref;
   var newtype$check#2: ref;
   var newtype$check#3: ref;
@@ -5452,6 +5456,10 @@ implementation {:smt_option "smt.arith.solver", "2"} {:verboseName "ChainingObje
     assume {:captureState "referrers.dfy(102,2): initial state"} true;
     $_reverifyPost := false;
     // ----- divided block before new; ----- C:\Users\mimayere\Documents\dafny\Source\IntegrationTests\TestFiles\LitTests\LitTest\referrers\referrers.dfy(102,3)
+    defass#this.x := false;
+    defass#this.y := false;
+    defass#this.tracking := false;
+    defass#this.tail := false;
     // ----- assignment statement ----- C:\Users\mimayere\Documents\dafny\Source\IntegrationTests\TestFiles\LitTests\LitTest\referrers\referrers.dfy(103,7)
     assume true;
     assume true;
@@ -5480,6 +5488,7 @@ implementation {:smt_option "smt.arith.solver", "2"} {:verboseName "ChainingObje
             $Box(#_System._tuple#2._#Make2($Box(this), $Box(_module.ChainingObject.x)))));
     }
 
+    defass#this.x := true;
     assume {:captureState "referrers.dfy(103,13)"} true;
     // ----- assignment statement ----- C:\Users\mimayere\Documents\dafny\Source\IntegrationTests\TestFiles\LitTests\LitTest\referrers\referrers.dfy(104,7)
     assume true;
@@ -5509,6 +5518,7 @@ implementation {:smt_option "smt.arith.solver", "2"} {:verboseName "ChainingObje
             $Box(#_System._tuple#2._#Make2($Box(this), $Box(_module.ChainingObject.y)))));
     }
 
+    defass#this.y := true;
     assume {:captureState "referrers.dfy(104,13)"} true;
     // ----- assignment statement ----- C:\Users\mimayere\Documents\dafny\Source\IntegrationTests\TestFiles\LitTests\LitTest\referrers\referrers.dfy(105,14)
     assume true;
@@ -5538,6 +5548,7 @@ implementation {:smt_option "smt.arith.solver", "2"} {:verboseName "ChainingObje
             $Box(#_System._tuple#2._#Make2($Box(this), $Box(_module.ChainingObject.tracking)))));
     }
 
+    defass#this.tracking := true;
     assume {:captureState "referrers.dfy(105,20)"} true;
     // ----- assignment statement ----- C:\Users\mimayere\Documents\dafny\Source\IntegrationTests\TestFiles\LitTests\LitTest\referrers\referrers.dfy(106,17)
     assume true;
@@ -5585,8 +5596,13 @@ implementation {:smt_option "smt.arith.solver", "2"} {:verboseName "ChainingObje
             $Box(#_System._tuple#2._#Make2($Box(this), $Box(_module.ChainingObject.tail)))));
     }
 
+    defass#this.tail := true;
     assume {:captureState "referrers.dfy(107,24)"} true;
     // ----- new; ----- C:\Users\mimayere\Documents\dafny\Source\IntegrationTests\TestFiles\LitTests\LitTest\referrers\referrers.dfy(102,3)
+    assert {:id "id249"} defass#this.x;
+    assert {:id "id250"} defass#this.y;
+    assert {:id "id251"} defass#this.tracking;
+    assert {:id "id252"} defass#this.tail;
     assume this != null && $Is(this, Tclass._module.ChainingObject?());
     assume !$Unbox(read($Heap, this, alloc)): bool;
     assume $Unbox(read($Heap, this, _module.ChainingObject.x)): ref == this.x;
